# Logistic Regression as a Neural Network

## Binary Classification
In a binary classification problem, the result is a discrete value output.

## Logistic Regression
Logistic regression is a learning algorithm used in a supervised learning problem when the output $y$ are all either zero or one. The goal of logistic regression is to minimize the error between its predictions and training data.

### Cat vs No-cat
Given an image represented by a feature vector ð‘¥, the algorithm will evaluate the probability of a cat being in that image.
$$
\text { Given } x , \hat { y } = P ( y = 1 | x ) , \text { where } 0 \leq \hat { y } \leq 1
$$
The parameters used in Logistic regression are:
- The input features vector: $x \in \mathbb { R } ^ { n _ { x } }$, where $n _ { x }$ is the number of features

- The training label: $y \in 0,1$

- The weights: $w \in \mathbb { R } ^ { n _ { x } }$, where $n _ { x }$ is the number of features

- The threshold: $b \in \mathbb { R }$

- The output: $\hat { y } = \sigma \left( w ^ { T } x + b \right)$

- Sigmoid function: $s = \sigma \left( w ^ { T } x + b \right) = \sigma ( z ) = \frac { 1 } { 1 + e ^ { - z } }$

$\left( w ^ { T } x + b \right)$ is a linear function $( a x + b )$, but since we are looking for a probability constraint between $[ 0,1 ] ,$ the sigmoid function is used.

## Logistic Regression Cost Function
To train the parameters $w$ and $b$, we need to define a cost function.

### Recap
$\hat { y } ^ { ( i ) } = \sigma \left( w ^ { T } x ^ { ( i ) } + b \right) ,$ where $\sigma \left( z ^ { ( i ) } \right) = \frac { 1 } { 1 + e ^ { - z ^ { ( i ) } } }$

Given $\left\{ \left( x ^ { ( 1 ) } , y ^ { ( 1 ) } \right) , \cdots , \left( x ^ { ( m ) } , y ^ { ( m ) } \right) \right\} ,$ we want $\hat { y } ^ { ( i ) } \approx y ^ { ( i ) }$

::: tip
$x ^ { ( i ) }$ : the i-th training example
:::

### Loss (error) function
The loss function measures the discrepancy between the prediction $\hat{y}^{(i)}$ and the desired output $y^{(i)}$.

In other words, the loss function computes the error for a single training example.

$\mathcal{L} \left( \hat { y } ^ { ( i ) } , y ^ { ( i ) } \right) = \frac { 1 } { 2 } \left( \hat { y } ^ { ( i ) } - y ^ { ( i ) } \right) ^ { 2 }$
  - We do not use this because of multiple minimums.

$\mathcal{L} \left( \hat { y } ^ { ( i ) } , y ^ { ( i ) } \right) = - \left( y ^ { ( i ) } \log \left( \hat { y } ^ { ( i ) } \right) + \left( 1 - y ^ { ( i ) } \right) \log \left( 1 - \hat { y } ^ { ( i ) } \right) \right)$
  - If $y ^ { ( i ) } = 1 : \mathcal{L} \left( \hat { y } ^ { ( i ) } , y ^ { ( i ) } \right) = - \log \left( \hat { y } ^ { ( i ) } \right)$ want be close to $0$, where $\log \left( \hat { y } ^ { ( i ) } \right)$ and $\hat { y } ^ { ( i ) }$ should be close to $1$
  - If $y ^ { ( i ) } = 0 : \mathcal{L} \left( \hat { y } ^ { ( i ) } , y ^ { ( i ) } \right) = - \log \left( 1 - \hat { y } ^ { ( i ) } \right)$ want be close to $0$, where $\log \left( 1 - \hat { y } ^ { ( i ) } \right)$ and $\hat { y } ^ { ( i ) }$ should be close to $0$

> Rafidah's effect:
> if $y=1$ we try to make $\hat{y}$ large and if $y=0$ we try to make $\hat{y}$ small.

::: tip

Interpret $\hat { y } = P ( y = 1 | x )$ and we get the function which matches the meaning:

$P ( y | x ) = \hat { y } ^ { y } ( 1 - \hat { y } ) ^ { ( 1 - y ) }$
  - $P ( y = 1 | x ) = \hat { y }$
  - $P ( y = 0 | x ) = 1 - \hat { y }$

$$
\begin{aligned}
\log \left[ P ( y | x ) \right] & = \log \left[ \hat { y } ^ { y } ( 1 - \hat { y } ) ^ { ( 1 - y ) } \right]\\
& = y \log ( \hat { y } ) + ( 1 - y ) \log ( 1 - \hat { y } )\\
& = - \mathcal{L} \left( \hat { y } , y \right)
\end{aligned}
$$

> minimizing the loss corresponds to maximizing the log of the probability.

:::

### Cost function
The cost function is the average of the loss function of the entire training set. We are going to find the parameters $w$ and $b$ that minimize the overall cost function.

$$
J ( w , b ) = \frac { 1 } { m } \sum _ { i = 1 } ^ { m } \mathcal{L} \left( \hat { y } ^ { ( i ) } , y ^ { ( i ) } \right) = - \frac { 1 } { m } \sum _ { i = 1 } ^ { m } \left[ y ^ { ( i ) } \log \left( \hat { y } ^ { ( i ) } \right) + \left( 1 - y ^ { ( i ) } \right) \log \left( 1 - \hat { y } ^ { ( i ) } \right) \right]
$$

::: tip

$$
\begin{aligned}
\log{[P(\text{labels in training set})]} & \xlongequal{\text{IID}} \log{\left[\prod _ { i = 1 } ^ { m } P \left( y ^ { ( i ) } | x ^ { ( i ) } \right)\right]}\\
& = \sum _ { i = 1 } ^ { m } \log \left[ P \left(y ^ { ( i ) } | x ^ { ( i ) } \right) \right]\\
& = - \sum _ { i = 1 } ^ { m } \mathcal{L} \left( \hat { y } ^ { ( i ) } , y ^ { ( l ) } \right)
\end{aligned}
$$

- IID: Independent and Identically Distributed

Use `maximnm likelihood estimation` to minimize the cost function.

$$
\text{Cost: } J(w,b) = \frac { 1 } { m } \sum _ { i = 1 } ^ { m } \mathcal{L} \left( \hat { y } ^ { ( i ) } , y ^ { ( i ) } \right)
$$

:::

## Gradient Descent
Want to find $w$, $b$ that minimize $J(w,b)$

```Pseudocode
Repeat{
	w := w - alpha * dw
	b := b - alpha * db
}
```

::: tip

$dw = \dfrac { \partial J ( w , b ) } { \partial w }$

$db = \dfrac { \partial J ( w , b ) } { \partial b }$

:::

## Computation graph
The computations of a neural network are organized in terms of a forward pass or a forward propagation step, in which we compute the output of the neural network, followed by a backward pass or back propagation step, which we use to compute gradients or compute derivatives. 

The computation graph explains why it is organized this way.

## Derivatives with a Computation Graph
It is used to do derivative calculations for the function $J$.
In calculus, it is called the `chain rule`.
So indeed, terminology of backpropagation if you want to compute the derivative of this final output variable with respect to v, then we've done one step of `backpropagation`.

- `dvar` = $\dfrac{\mathrm{d} \text{FinalOutputVar}}{\mathrm{d} \text{var}}$

## Logistic Regression Gradient Descent
Using the computation graph is a little bit of an overkill for deriving gradient descent for logistic regression.

### Recap
$z = w ^ { T } x + b$

$\hat { y } = a = \sigma ( z ) = \frac { 1 } { 1 + e ^ { - z } }$

$\mathcal { L } ( a , y ) = - ( y \log ( a ) + ( 1 - y ) \log ( 1 - a ) )$

### Back propagation
`da` = $\dfrac{\mathrm{d}\mathcal{L}}{\mathrm{d}a} = - \dfrac { y } { a } + \dfrac { 1 - y } { 1 - a }$

`dz` = $\dfrac{\mathrm{d}\mathcal{L}}{\mathrm{d}z} = \dfrac{\mathrm{d}\mathcal{L}}{\mathrm{d}a} \cdot \dfrac{\mathrm{d}\mathcal{a}}{\mathrm{d}z} = a-y$

`dw_1` = $\dfrac{\mathrm{d}\mathcal{L}}{\mathrm{d}w_1} = x_1 \cdot$`dz`

`dw_2` = $\dfrac{\mathrm{d}\mathcal{L}}{\mathrm{d}w_2} = x_2 \cdot$`dz`

`db` = $\dfrac{\mathrm{d}\mathcal{L}}{\mathrm{d}b}$ = `dz`

## Gradient Descent on m Examples
$J ( w , b ) = \dfrac { 1 } { m } \displaystyle\sum _ { i = 1 } ^ { m } \mathcal{L} \left( a ^ { ( i ) } , y ^ { ( i ) } \right)$

$a ^ { ( i ) } = \hat { y } ^ { ( i ) } = \sigma \left( z ^ { ( i ) } \right) = \sigma \left( w ^ { T } x ^ { ( i ) } + b \right)$

$\dfrac { \partial } { \partial w _ { 1 } } J ( w , b ) = \dfrac { 1 } { m } \displaystyle\sum _ { i = 1 } ^ { m } \dfrac { \partial } { \partial w _ { 1 } } \mathcal{L} \left( a ^ { ( i ) } , y ^ { ( i ) } \right) = \dfrac { 1 } { m } \displaystyle\sum _ { i = 1 } ^ { m } \mathrm{d} w_1^{(i)}$